Completed the agreement proof in AbstractMultiPaxos.thy

Isabelle2/AbstractMultiPaxos.thy
@@ -1,350 +1,244 @@
 theory AbstractMultiPaxos
-imports Main LinorderOption "~~/src/HOL/Library/FSet"
+imports Main LinorderOption "~~/src/HOL/Library/FSet" Quorums
+  "/home/nano/Documents/IO-Automata/IOA_Automation"  "~~/src/HOL/Eisbach/Eisbach_Tools"
+  "/home/nano/Documents/IO-Automata/Simulations" BallotArrays
 begin
 
-text {* 
-The use of statespaces and FinFuns hampers Sledgehammer... 
-Which feature does the most?
-Why not interpret the locale to get rid of the statespace before the proofs?
-Why not have two versions, one with normal functions and the other with FinFuns, then prove a refinement mapping? *}
-
-datatype ('v,'a,'l) p_action =
+datatype ('v,'a,'l) amp_action =
   Propose 'v
-| Learn 'v 'l
-| Vote 'a
-| JoinBallot nat 'a
-| StartBallot nat
+| Learn nat 'v 'l
+| Vote 'a "'a fset" nat 'v 
+  -- {* an acceptor votes in a ballot according to a quorum *}
+| JoinBallot 'a nat
 
-record ('v,'a,'b) abs_multi_paxos_state =
-  propCmd :: "'v set"
-  ballot :: "'a \<Rightarrow> nat \<Rightarrow> 'b option"
-  vote :: "'a \<Rightarrow> nat \<Rightarrow> 'b \<Rightarrow> 'v option"
-
+record ('v,'a) amp_state =
+  propCmd :: "'v fset"
+  ballot :: "'a \<Rightarrow> nat option"
+  vote :: "nat \<Rightarrow> 'a \<Rightarrow> nat \<Rightarrow> 'v option"
 
 text {* We give all the parameters in order to fix their type. Also fixed ballots to be nat. *}
-locale abs_multi_paxos = 
-  fixes acceptors::"'a fset" and learners::"'l fset" and quorums::"'a fset fset"
-  assumes "acceptors \<noteq> {||}"
-    and "learners \<noteq> {||}"
-    and "\<And> q1 q2 . \<lbrakk>q1 |\<in>| quorums; q2 |\<in>| quorums\<rbrakk> \<Longrightarrow> q1 |\<inter>| q2 \<noteq> {||}"
-    and "\<And> q . q |\<in>| quorums \<Longrightarrow> q |\<subseteq>| acceptors"
-    and "quorums \<noteq> {||}"
+locale abs_multi_paxos = IOA + quorums +
+  fixes learners::"'l fset"
+  assumes "learners \<noteq> {||}"
 begin
 
-definition conservative where
-  "conservative s b \<equiv> \<forall> a1 . \<forall> a2 . \<forall> i . a1 |\<in>| acceptors \<and> a2 |\<in>| acceptors \<longrightarrow> (
-    let v1 = vote s a1 i b; v2 = vote s a2 i b in
-      (v1 \<noteq> None \<and> v2 \<noteq> None) \<longrightarrow> v1 = v2)"
+definition amp_asig where
+  "amp_asig \<equiv>
+    \<lparr> inputs = { Propose c | c . True},
+      outputs = { Learn i v l | i v l . l |\<in>| learners},
+      internals = {Vote a i q b | a i b q . a |\<in>| acceptors} \<union> {JoinBallot a b | a b . a |\<in>| acceptors}\<rparr>"
 
-definition conservative_array where
-  "conservative_array r \<equiv> \<forall> b . conservative r b"
+definition amp_start where
+  "amp_start \<equiv> {\<lparr>propCmd = {||}, ballot = (\<lambda> a . None), vote = (\<lambda> i a b . None) \<rparr>}"
 
-text {* Here the max is the one from Lattices_Big *}
+definition propose where
+  "propose c r r' \<equiv> (r' = r\<lparr>propCmd := (propCmd r) |\<union>| {|c|}\<rparr>)"
 
-definition max_voted_round where
-  "max_voted_round s a i bound \<equiv> Max {b . vote s i a b \<noteq> None \<and> b \<le> bound}"
-  
-definition max_voted_round_q where
-  "max_voted_round_q s i q bound \<equiv> 
-    if \<exists> b a . a |\<in>| q \<and> b \<le> bound \<and> vote s a i b \<noteq> None
-    then Some (Max {b . \<exists> a . a |\<in>| q \<and> b \<le> bound \<and> vote s a i b \<noteq> None})
-    else None"
+definition join_ballot where
+  "join_ballot a b s s' \<equiv> 
+    a |\<in>| acceptors \<and> Some b > (ballot s a) \<and> s' = s\<lparr>ballot := (ballot s)(a := Some b)\<rparr>"
 
-lemma finite_voted_bals:"finite {b::nat . \<exists> a . a |\<in>| q \<and> b \<le> bound \<and> vote s i a b \<noteq> None}"
-  (is "finite ?S")
-proof -
-  have "?S \<subseteq> {b . b \<le> bound}"
-    by auto
-  moreover have "finite {b . b \<le> bound}" by simp
-  ultimately show ?thesis
-  by (metis (no_types, lifting) finite_subset) 
-qed
+abbreviation proved_safe_at where 
+  -- {* v is proved safe in instance i at ballot b by quorum q *}
+  "proved_safe_at s i q b v \<equiv> ballot_array.proved_safe_at  (vote s i) q b v"
+abbreviation conservative_at where 
+  "conservative_at s i \<equiv> ballot_array.conservative_array (vote s i) acceptors"
 
-lemma max_voted_round_none:
-  assumes "a |\<in>| q" and "(b::nat) \<le> bound" 
-  and "max_voted_round_q r i q bound = None \<or> b > the (max_voted_round_q r i q bound)"
-  shows "vote r a i b = None"
-proof (cases "max_voted_round_q r i q bound")
-case None 
-  thus ?thesis using assms(1,2)
-  by (auto simp add:max_voted_round_q_def split:split_if_asm)
-next
-  case (Some b\<^sub>m\<^sub>a\<^sub>x)
-  with this obtain a2 b2 v where "a2 |\<in>| q \<and> b2 \<le> bound \<and> vote r a2 i b2 = Some v"
-  by (auto simp add:max_voted_round_q_def split:split_if_asm)
-  hence "{b . \<exists> a . a |\<in>| q \<and> b \<le> bound \<and>  vote r a i b \<noteq> None} \<noteq> {}" by auto
-  with this obtain b2 a2 where "a2 |\<in>| q \<and> b2 \<le> bound \<and>  vote r a2 i b2 \<noteq> None"
-    by auto
-  moreover note finite_voted_bals
-  moreover have "b > Max {b . \<exists> a . a |\<in>| q \<and> b \<le> bound \<and>  vote r a i b \<noteq> None}" using Some assms(3)
-    by (auto simp add:max_voted_round_q_def split:split_if_asm)
-  ultimately
-  show ?thesis
-    by (smt Max_ge assms(1) assms(2) finite_nat_set_iff_bounded_le leD mem_Collect_eq) 
-qed
+definition do_vote where
+  "do_vote a i q v s s' \<equiv> a |\<in>| acceptors \<and> (case ballot s a of None \<Rightarrow> False | Some b \<Rightarrow> 
+        proved_safe_at s i q b v 
+        \<and> q |\<in>| quorums
+        \<and> (\<forall> a2 . a2 |\<in>| q \<longrightarrow> ballot s a2 \<ge> Some b)
+        \<and> conservative_at s' i
+        \<and> vote s i a b = None 
+        \<and> s' = s\<lparr>vote := (vote s)(i := (vote s i)(a := 
+            (vote s i a)(b := Some v)))\<rparr>)"
 
-lemma max_voted_round_some :
-  assumes "max_voted_round_q s i q (bound::nat) = Some (b::nat)"
-  obtains a where "a |\<in>| q" and "vote s a i b \<noteq> None" and "b \<le> bound"
-proof -
-  from assms have "b = Max {b . \<exists> a . a |\<in>| q \<and> b \<le> bound \<and> vote s a i b \<noteq> None}"
-    by (auto simp add:max_voted_round_q_def split:split_if_asm)
-  moreover note finite_voted_bals
-  moreover obtain a2 b2 where "a2 |\<in>| q \<and> b2 \<le> bound \<and> vote s a2 i b2 \<noteq> None"
-    using assms apply (auto simp add:max_voted_round_q_def)
-      by (metis (no_types, hide_lams) option.simps(3)) 
-  ultimately show ?thesis using that
-  by (smt Max_in empty_iff finite_nat_set_iff_bounded_le mem_Collect_eq) 
-qed
- 
-definition max_vote where
-  "max_vote s i q bound \<equiv>
-    case max_voted_round_q s i q bound of
-      None \<Rightarrow> None
-    | Some b \<Rightarrow> 
-        let max_voter = (SOME a . a |\<in>| q \<and> vote s a i b \<noteq> None)
-        in vote s max_voter i b"
+abbreviation chosen where 
+  "chosen s i v \<equiv> ballot_array.chosen (vote s i) quorums v"
+definition learn where
+  "learn l i v s s' \<equiv> chosen s i v \<and> s = s'"
 
-lemma max_vote_some_prop:
-  assumes "max_vote s i q (bound::nat) = Some v"
-  obtains a b\<^sub>m\<^sub>a\<^sub>x where "vote s a i b\<^sub>m\<^sub>a\<^sub>x = max_vote s i q bound" and "a |\<in>| q"
-  and "\<And> a2 b2 . \<lbrakk>a2 |\<in>| q; b2 > b\<^sub>m\<^sub>a\<^sub>x; b2 \<le> bound\<rbrakk> \<Longrightarrow> vote s a2 i b2 = None"
-  and "b\<^sub>m\<^sub>a\<^sub>x \<le> bound"
-proof -
-  from assms obtain b\<^sub>m\<^sub>a\<^sub>x where 0:"max_voted_round_q s i q bound = Some (b\<^sub>m\<^sub>a\<^sub>x::nat)"
-    by (auto simp add:max_vote_def) (metis (lifting) not_None_eq option.simps(4)) 
-  with max_voted_round_some obtain a where
-    "a |\<in>| q" and "vote s a i  b\<^sub>m\<^sub>a\<^sub>x \<noteq> None" (is "?bmax \<noteq> None") and 1:"b\<^sub>m\<^sub>a\<^sub>x \<le> bound" by metis
-  hence 
-    "let a2 = SOME a . a |\<in>| q \<and> ?bmax \<noteq> None in a2 |\<in>| q \<and> ?bmax \<noteq> None"
-      by (metis (mono_tags, lifting) someI_ex)
-  moreover have "\<And> a2 b2 . \<lbrakk>a2 |\<in>| q; b2 \<le> bound; b2 > b\<^sub>m\<^sub>a\<^sub>x\<rbrakk> \<Longrightarrow> vote s a2 i b2 = None" 
-    using max_voted_round_none by (metis "0" option.sel)  
-  moreover have "max_vote s i q bound = vote s (SOME a . a |\<in>| q \<and> vote s a i b\<^sub>m\<^sub>a\<^sub>x \<noteq> None) i b\<^sub>m\<^sub>a\<^sub>x"
-    using 0 by (auto simp add:max_vote_def)
-  ultimately show ?thesis using that 1
-    by (smt \<open>a |\<in>| q\<close> someI_ex)
-qed
+(* Here it's better to have all existentially quantified parameters in the action itself, in
+  order to avoid annoying quantifiers. *)
+fun amp_trans_fun  where
+  "amp_trans_fun r (Propose c) r' = propose c r r'"
+| "amp_trans_fun r (JoinBallot a b) r' = join_ballot a b r r'"
+| "amp_trans_fun r (Vote a q i v) r' = do_vote a i q v r r'"
+| "amp_trans_fun r (Learn i v l) r' = learn l i v r r'"
 
-lemma max_vote_none_prop:
-  assumes "max_vote s i q bound = None"
-  shows "\<And> a (b::nat) . \<lbrakk>a |\<in>| q; b \<le> bound\<rbrakk> \<Longrightarrow> vote s a i b = None"
-using assms
-apply (simp add:max_vote_def split add:option.split_asm)
-    apply (metis max_voted_round_none)
-  apply (smt max_voted_round_some not_None_eq someI_ex)
-done
-  
-definition proved_safe_at where
-  "proved_safe_at r i Q b v \<equiv>
-    case b of 0 \<Rightarrow> True
-  | Suc c \<Rightarrow> (case (max_vote r i Q c) of (* note that here c is b-1 *)
-      None \<Rightarrow> True
-    | Some v' \<Rightarrow> v = v')"
+definition amp_trans where
+  "amp_trans \<equiv> { (r,a,r') . amp_trans_fun r a r'}"
 
-definition chosen_at where
-  "chosen_at r i v b \<equiv> \<exists> q . q |\<in>| quorums \<and> (\<forall> a . a |\<in>| q \<longrightarrow> (vote r) a i b = (Some v))"
-
-definition chosen where
-  "chosen r i v \<equiv> \<exists> b . chosen_at r i v b"
-  
-definition choosable where
-  "choosable r i v b \<equiv>
-    \<exists> q . q |\<in>| quorums \<and> (\<forall> a . a |\<in>| q \<longrightarrow> (
-      (ballot r a i) > Some b \<longrightarrow> (vote r) a i b = Some v))"
-
-definition safe_at where
-  "safe_at r i v b \<equiv>
-    (\<forall> b2 . \<forall> v2 .
-      ((b2 < b \<and> choosable r i v2 b2) \<longrightarrow> (v = v2)))"
-
-definition safe where
-  "safe r \<equiv> \<forall> i . \<forall> b . \<forall> a . a |\<in>| acceptors \<longrightarrow> 
-    (let vote = (vote r) a i b in (vote \<noteq> None \<longrightarrow> safe_at r i (the vote) b))"
-  
-definition well_formed where
-  "well_formed r  \<equiv> \<forall> i a b . a |\<in>| acceptors \<and> (ballot r) a i < b  
-    \<longrightarrow> (vote r) a i (the b) = None"
-
-lemma "safe_at r i v (bot::nat)"
-by (auto simp add:safe_at_def)
-
-lemma chosen_at_is_choosable:
-  assumes "chosen_at r i v b"
-  shows "choosable r i v b" using assms
-  by (auto simp add:chosen_at_def choosable_def)
-
-lemma safe_at_prec:
-  assumes "safe_at r i v (b::nat)" and "b2 < b"
-  shows "safe_at r i v b2"
-  using assms by (meson order.strict_trans safe_at_def)
-
-lemma quorum_inter_witness:
-  assumes "q1 |\<in>| quorums" and "q2 |\<in>| quorums"
-  obtains a where "a |\<in>| q1" and "a |\<in>| q2"
-  using assms abs_multi_paxos_axioms abs_multi_paxos_def
-  by (metis all_not_fin_conv finter_iff)
-
-lemma quorum_vote:
-  assumes "q1 |\<in>| quorums" and "q2 |\<in>| quorums"
-  and "\<And> a . a |\<in>| q1 \<Longrightarrow> vote r a i b = Some v1"
-  and "\<And> a . a |\<in>| q2 \<Longrightarrow> vote r a i b = Some v2"
-  shows "v1 = v2"
-proof -
-  obtain a where "a |\<in>| q1" and "a |\<in>| q2"
-  proof -
-    have "q1 |\<inter>| q2 \<noteq> {||}" using assms(1,2)
-      by (metis abs_multi_paxos_axioms abs_multi_paxos_def)
-    hence "\<exists> a . a |\<in>| q1 \<and> a |\<in>| q2"
-      by (metis assms(1) assms(2) quorum_inter_witness) 
-    with that show ?thesis by auto
-  qed
-  thus ?thesis using assms(3,4) by force
-qed
-
-lemma chosen_at_same:
-  assumes "chosen_at r i v1 b1" and "chosen_at r i v2 b1"
-  shows "v1 = v2" using quorum_vote assms
-  by (auto simp add:chosen_at_def) fast
-
-lemma all_choosable_no_safe:
-  assumes "\<And> (v::'v) . choosable r i v b"
-  and "safe_at r i v (Suc b)" and "(v1::'v) \<noteq> v2"
-  shows False using assms 
-  by (auto simp add:safe_at_def)(metis lessI)
-
-lemma safe_is_safe:
-  assumes "safe r" and "chosen r i v\<^sub>1" and "chosen r i v\<^sub>2"
-  shows "v\<^sub>1 = v\<^sub>2"
-  -- {* This follows the proof of Proposition 1 from "Generalized Consensus and Paxos" *}
-proof -
-  text {* The main argument as a lemma to avoid repetitions*}
-  { fix b\<^sub>1 b\<^sub>2 v\<^sub>1 v\<^sub>2
-    assume 1:"chosen_at r i v\<^sub>1 b\<^sub>1" and 2:"chosen_at r i v\<^sub>2 b\<^sub>2"
-    with this obtain q\<^sub>1 and q\<^sub>2 where 3:"\<And> a . a |\<in>| q\<^sub>1 \<Longrightarrow> vote r a i b\<^sub>1 = (Some v\<^sub>1)" 
-    and 4:"\<And> a . a |\<in>| q\<^sub>2 \<Longrightarrow> (vote r) a i b\<^sub>2 = (Some v\<^sub>2)" and 5:"q\<^sub>1 |\<in>| quorums" and 6:"q\<^sub>2 |\<in>| quorums"
-    by (auto simp add:chosen_at_def)
-    have "v\<^sub>1 = v\<^sub>2" if "b\<^sub>1 < b\<^sub>2"
-    proof -
-      have 9:"choosable r i v\<^sub>1 b\<^sub>1" using 1 chosen_at_is_choosable by fast
-      have 10:"safe_at r i v\<^sub>2 b\<^sub>2"
-      proof -
-        obtain a where "a |\<in>| q\<^sub>2" using 6 by (metis quorum_inter_witness)
-        with this assms(1) 4 6 have "safe_at r i (the (vote r a i b\<^sub>2)) b\<^sub>2" 
-          using abs_multi_paxos_axioms abs_multi_paxos_def apply auto (* Prood reconstruction fails without calling auto first *)
-            by (metis abs_multi_paxos_def fset_rev_mp option.discI option.sel safe_def)
-        moreover have "the (vote r a i b\<^sub>2) = v\<^sub>2" using `a |\<in>| q\<^sub>2` 4 by force
-        ultimately show ?thesis by auto
-      qed
-      thus ?thesis using 9 10 assms(1) that by (metis safe_at_def)
-    qed }
-  note main = this
-  obtain b\<^sub>1 and b\<^sub>2 where 1:"chosen_at r i v\<^sub>1 b\<^sub>1" and 2:"chosen_at r i v\<^sub>2 b\<^sub>2" using assms(2,3)
-  by (auto simp add:chosen_def)
-  have ?thesis if "b\<^sub>1 = b\<^sub>2" by (metis "1" "2" chosen_at_same that)
-  moreover
-  have ?thesis if "b\<^sub>1 < b\<^sub>2" using main 1 2 that by blast
-  moreover 
-  have ?thesis if "b\<^sub>2 < b\<^sub>1" using main 1 2 that by blast
-  ultimately show ?thesis by fastforce
-qed
-
-text {* The main lemma *}
-
-lemma proved_safe_is_safe:
-  assumes "safe s" and "q |\<in>| quorums"
-  and "\<And> a . a |\<in>| q \<Longrightarrow> ballot s a n \<ge> Some i"
-  and "proved_safe_at s n q i v" and "conservative_array s"
-  shows "safe_at s n v (i::nat)"
-proof (cases "i = 0")
-  case True thus ?thesis
-    by (metis not_less0 safe_at_def) 
-next
-  case False
-  consider 
-    (a) k a
-      where "a |\<in>| q" and "vote s a n k = Some v" and "k < i"
-      and "\<And> a\<^sub>2 l . \<lbrakk>a\<^sub>2 |\<in>| q; k < l; l < i\<rbrakk> \<Longrightarrow> vote s a\<^sub>2 n l = None"
-  | (b) "\<And> a k . \<lbrakk>a |\<in>| q; k < i\<rbrakk>  \<Longrightarrow> vote s a n k = None"
-  proof (cases "max_vote s n q (i-1)")
-    case None 
-    hence "\<And> a k . \<lbrakk>a |\<in>| q; k < i\<rbrakk>  \<Longrightarrow> vote s a n k = None" 
-      using False by (metis Suc_diff_eq_diff_pred Suc_leI diff_is_0_eq gr0I max_vote_none_prop)
-    thus ?thesis using that by auto
-  next
-    case (Some v') 
-    with this obtain k a where "a |\<in>| q" and "vote s a n k = Some v" and "k < i"  
-      and "\<And> a\<^sub>2 l . \<lbrakk>a\<^sub>2 |\<in>| q; k < l; l < i\<rbrakk> \<Longrightarrow> vote s a\<^sub>2 n l = None"
-      using False assms(4)
-      by (simp add:proved_safe_at_def)
-      (smt False Nitpick.case_nat_unfold Some Suc_pred less_Suc_eq_le max_vote_some_prop option.case_eq_if option.sel option.simps(3)) 
-    thus ?thesis using that by auto
-  qed
-  thus ?thesis
-  proof (cases)
-    case b
-    { fix j v
-      assume 1:"j < i"  and 2:"choosable s n v j"
-      from 2 obtain q2 where 3:"q2 |\<in>| quorums" and 4:"\<And> a . a |\<in>| q2 \<Longrightarrow>
-        (ballot s a n) > Some j \<Longrightarrow> (vote s) a n j = Some v"
-        by (auto simp add:choosable_def)
-      from 3 assms(2) obtain a where 5:"a |\<in>| q" and 6:"a |\<in>| q2"
-        using quorum_inter_witness by metis
-      have 9:"vote s a n j = Some v"
-        by (metis (no_types, hide_lams) "1" "4" "5" "6" assms(3) less_def less_o.simps(4) not_le order_trans) 
-      from b have False by (metis "1" "5" "9" option.distinct(1)) }
-    thus ?thesis by (auto simp add:safe_at_def)
-  next
-    case a
-    have "v' = v" if "choosable s n v' j" and "j < i" for j v'
-    proof -
-      consider (aa) "j < k" | (bb) "j = k" | (cc) "k < j" by fastforce
-      hence ?thesis
-      proof cases
-        case aa
-        have "a |\<in>| acceptors"
-          by (metis abs_multi_paxos_axioms abs_multi_paxos_def a(1) assms(2) fset_mp) 
-        hence "safe_at s n v k" using  assms(1)
-          by (metis a(2) option.discI option.sel safe_def)
-        with aa show ?thesis using that by (metis safe_at_def) 
-      next
-        case cc
-        from that obtain q2 where 3:"q2 |\<in>| quorums" and 4:"\<And> a . a |\<in>| q2 \<Longrightarrow>
-          (ballot s a n) > Some j \<Longrightarrow> (vote s) a n j = Some v'"
-          by (auto simp add:choosable_def)
-        from 3 assms(2) obtain a2 where 5:"a2 |\<in>| q" and 6:"a2 |\<in>| q2" 
-          using quorum_inter_witness by metis
-        have 8:"vote s a2 n j = Some v'"
-          by (metis (mono_tags, lifting) "4" "5" "6" assms(3) leD leI less_eq_def less_eq_o.simps(3) order_trans that(2)) 
-        show ?thesis using a(4) 5 that(2) 8 cc by (metis option.distinct(1))
-      next
-        case bb (* Here we probably need the fact that the array is conservative: *)
-        have 1:"vote s a n k = Some v" if "a |\<in>| acceptors" and " vote s a n k \<noteq> None"  for a using that assms(5) 
-          by (auto simp add:conservative_array_def conservative_def)
-            (metis (no_types, hide_lams) abs_multi_paxos_axioms abs_multi_paxos_def a(1) a(2) assms(2) option.inject order.not_eq_order_implies_strict pfsubsetD)  
-        from that obtain q2 where 3:"q2 |\<in>| quorums" and 4:"\<And> a . a |\<in>| q2 \<Longrightarrow>
-          (ballot s a n) > Some j \<Longrightarrow> (vote s) a n j = Some v'"
-          by (auto simp add:choosable_def)
-        from 3 assms(2) obtain a2 where 5:"a2 |\<in>| q" and 6:"a2 |\<in>| q2" 
-          using quorum_inter_witness by metis
-        have 7:"ballot s a2 n \<ge> Some k"
-          by (metis "5" a(3) assms(3) less_eq_def less_eq_o.simps(3) less_imp_le order_trans)
-        have 8:"a2 |\<in>| acceptors"
-          by (metis "5" abs_multi_paxos_axioms abs_multi_paxos_def assms(2) order.not_eq_order_implies_strict pfsubsetD) 
-        have 9:"vote s a2 n k = Some v"
-          by (metis "1" "4" "5" "6" "7" "8" assms(3) bb leD less_eq_def less_eq_o.simps(3) option.discI order.not_eq_order_implies_strict that(2))
-        show ?thesis
-          by (metis "4" "5" "6" "7" "9" antisym_conv2 assms(3) bb leD less_eq_def less_eq_o.simps(3) option.sel that(2)) 
-      qed
-      thus ?thesis by (auto simp add:safe_at_def)
-    qed
-    thus ?thesis
-    by (metis safe_at_def) 
-  qed 
-qed
-
-section {* The I/O-automaton *}
+definition amp_ioa where
+  "amp_ioa \<equiv> \<lparr>ioa.asig = amp_asig, start = amp_start, trans = amp_trans\<rparr>"
 
 end
+
+locale amp_proof = IOA + abs_multi_paxos acceptors quorums learners for acceptors :: "'a fset" 
+  and quorums and learners :: "'l fset" +
+  fixes the_ioa :: "(('v,'a)amp_state, ('v,'a,'l)amp_action) ioa"
+  defines "the_ioa \<equiv> amp_ioa"
+begin
+
+lemmas amp_ioa_defs =  
+   is_trans_def actions_def amp_trans_def amp_start_def
+   externals_def amp_ioa_def amp_asig_def
+
+declare amp_ioa_defs[inv_proofs_defs]
+declare the_ioa_def[inv_proofs_defs]
+
+declare propose_def[simp] join_ballot_def[simp] do_vote_def[simp]
+  learn_def[simp]
+
+lemma vote_one_inst_only:
+  assumes "do_vote a i q v s s'" and "i \<noteq> j"
+  shows "vote s j a = vote s' j a "
+using assms
+apply auto
+    apply (case_tac "ballot s a")
+apply auto
+done
+
+lemma vote_ballot_unch:
+  assumes "do_vote a i q v s s'"
+  shows "ballot s = ballot s'"
+using assms by (auto split add:option.split_asm)
+
+declare ballot_array.conservative_array_def[inv_proofs_defs]
+abbreviation conservative_array where 
+"conservative_array s \<equiv>  \<forall> i . conservative_at s i"
+lemma conservative_inductive:
+  "invariant the_ioa conservative_array"
+apply (try_solve_inv2 inv_proofs_defs:inv_proofs_defs invs:invs)
+    apply (force simp add:ballot_array.conservative_def)
+  apply (case_tac a)
+        apply (force simp add:inv_proofs_defs)
+      apply (force simp add:inv_proofs_defs)
+    defer
+    apply (force simp add:inv_proofs_defs)
+  apply (match premises in R[thin]:"reachable ?ioa ?s" \<Rightarrow> \<open>-\<close>)
+  subgoal premises prems for s t act a q i v using prems
+  proof -
+    from prems(2,3)
+    obtain b where 1:"a |\<in>| acceptors" and 2:"ballot s a = Some b" 
+    and 3:"proved_safe_at s i q b v"
+    and 6:"ballot_array.conservative_array  (vote t i) acceptors"
+    and 4:"vote s i a b = None" and 5:"t = s\<lparr>vote := (vote s)(i := (vote s i)(a := (vote s i a)(b := Some v)))\<rparr>"
+        apply (case_tac "ballot s a")
+          by (auto simp add:inv_proofs_defs)
+    show "conservative_array t"
+    proof (auto simp add: ballot_array.conservative_array_def)
+      fix j b
+      have "ballot_array.conservative (vote t j) acceptors b" if "i \<noteq> j"
+      proof -
+        have "ballot_array.conservative (vote s j) acceptors b" using prems(1)
+          by (auto simp add: ballot_array.conservative_array_def ballot_array.conservative_def)
+        thus ?thesis using that 5 by (auto simp add: ballot_array.conservative_def)
+      qed
+      moreover
+      have "ballot_array.conservative (vote t j) acceptors b" if "i = j"
+        using 6 that by auto (metis ballot_array.conservative_array_def)
+      ultimately show "ballot_array.conservative (vote t j) acceptors b" by auto
+    qed
+  qed 
+done
+declare conservative_inductive[invs]
+
+abbreviation safe_at where "safe_at s i \<equiv> ballot_array.safe_at (ballot s) (vote s i) quorums"
+lemma safe_mono:
+  assumes "safe_at s i v b" and "s \<midarrow>a\<midarrow>the_ioa\<longrightarrow> t"
+  shows "safe_at t i v b" using assms
+apply (cases a)
+         (* propose, learn *)
+        apply (auto simp add:inv_proofs_defs ballot_array.safe_at_def ballot_array.choosable_def)[2]
+    defer 
+    (* join_ballot *)
+    apply (simp add:inv_proofs_defs ballot_array.safe_at_def ballot_array.choosable_def)[1]
+    apply (metis less_def order.strict_trans)
+  (* vote *)
+  apply (simp add:inv_proofs_defs ballot_array.safe_at_def ballot_array.choosable_def split add:option.split_asm)
+  apply (metis neq_iff)
+done
+
+abbreviation safe where "safe s \<equiv> \<forall> i . ballot_array.safe (ballot s) (vote s i) quorums acceptors"
+lemma safe_inv:
+  "invariant the_ioa safe"
+apply(rule invariantI)
+    apply (force simp add:ballot_array.safe_def inv_proofs_defs)
+  apply instantiate_invs_2
+  apply (case_tac a)
+        (* propose *)
+        apply (force simp add:ballot_array.safe_def inv_proofs_defs ballot_array.safe_at_def ballot_array.choosable_def)
+      (* learn *)
+      apply (force simp add:ballot_array.safe_def inv_proofs_defs ballot_array.safe_at_def ballot_array.choosable_def)
+    (* vote *)
+    subgoal premises prems for s t act a q i v
+    proof (auto simp add:ballot_array.safe_def Let_def split add:option.split)
+      fix j b a\<^sub>2 v\<^sub>2
+      assume 1:"a\<^sub>2 |\<in>| acceptors" and 2:"vote t j a\<^sub>2 b = Some v\<^sub>2"
+      have l:"safe_at t j v\<^sub>2 b" if  "vote s j a\<^sub>2 b = vote t j a\<^sub>2 b"
+      proof -
+        have "safe_at s j v\<^sub>2 b" using that 1 2 prems(1) by (simp add:ballot_array.safe_def split add:option.split_asm)
+        thus ?thesis using prems(2) safe_mono by blast
+      qed
+      show "safe_at t j v\<^sub>2 b"
+      proof (cases "i = j \<and> a\<^sub>2 = a")
+      case False
+        have "vote s j a\<^sub>2 b = vote t j a\<^sub>2 b" using False prems(2,5) vote_one_inst_only
+          by (auto simp add:is_trans_def the_ioa_def amp_ioa_def amp_trans_def split add:option.split_asm)
+        with l show ?thesis by auto
+      next
+      case True
+        have 6:"do_vote a\<^sub>2 j q v s t" using prems(2,5) 1 True by (auto simp add:inv_proofs_defs)
+        with this obtain b\<^sub>2 where 3:"ballot s a\<^sub>2 = Some b\<^sub>2" and 4:"proved_safe_at s j q b\<^sub>2 v"
+        and 5:"t = s\<lparr>vote := (vote s)(j := (vote s j)(a\<^sub>2 := (vote s j a\<^sub>2)(b\<^sub>2 := Some v)))\<rparr>"
+        and 7:"\<And> a2 . a2 |\<in>| q \<Longrightarrow> ballot s a2 \<ge> Some b\<^sub>2" and 8:"q |\<in>| quorums"
+          by (auto split add:option.split_asm)
+        have ?thesis if "b \<noteq> b\<^sub>2"
+        proof -
+          have "vote s j a\<^sub>2 b = vote t j a\<^sub>2 b" using 5
+            by (smt amp_state.ext_inject amp_state.surjective amp_state.update_convs(3) fun_upd_apply that) 
+          with l show ?thesis by auto
+        qed
+        moreover have ?thesis if "b = b\<^sub>2"
+        proof -
+          have "v = v\<^sub>2" using that True
+            by (smt "2" "5" amp_state.ext_inject amp_state.surjective amp_state.update_convs(3) fun_upd_apply map_upd_Some_unfold)
+          hence 9:"vote t j a\<^sub>2 b = Some v\<^sub>2" using 5 that by force
+          hence "safe_at s j v\<^sub>2 b\<^sub>2" 
+            using ballot_array_props.proved_safe_is_safe[of quorums acceptors "ballot s" "(vote s j)" q b\<^sub>2 v] 4 3 7 8 prems(1,3) that `v = v\<^sub>2`
+            by auto (metis ballot_array_props_def quorums_axioms)
+          with safe_mono prems(2) that True show ?thesis by blast
+        qed
+        ultimately show ?thesis by auto
+      qed
+    qed
+  (* join_ballot *)
+  subgoal premises prems for s t act a b
+  proof (auto simp add:ballot_array.safe_def split add:option.split)
+    fix i b\<^sub>2 a\<^sub>2 v
+    assume "vote t i a\<^sub>2 b\<^sub>2 = Some v" and "a\<^sub>2 |\<in>| acceptors"
+    note 1 = this
+    have 2:"vote t i a\<^sub>2 b\<^sub>2 = vote s i a\<^sub>2 b\<^sub>2" using prems(2,5) by (auto simp add:inv_proofs_defs)
+    hence 3:"safe_at s i v b\<^sub>2" using 1 prems(1)
+      by (metis ballot_array.safe_def option.simps(5)) 
+    with safe_mono prems(2,5)
+    show "safe_at t i v b\<^sub>2" apply (auto simp add:inv_proofs_defs)
+      by (metis amp_proof.safe_mono amp_proof_axioms amp_state.select_convs(3) amp_state.simps(2) amp_state.surjective amp_state.update_convs(2) prems(2) the_ioa_def) 
+  qed
+done
+declare safe_inv[invs]
+
+definition agreement where 
+  "agreement s \<equiv> \<forall> v w i . chosen s i v \<and> chosen s i w \<longrightarrow> v = w"
+lemma agreement:"invariant the_ioa agreement"
+apply(rule invariantI)
+    apply(auto simp add: inv_proofs_defs agreement_def ballot_array.chosen_def ballot_array.chosen_at_def)[1]
+    apply (metis fempty_iff quorum_inter_witness)
+  apply instantiate_invs_2
+  apply (insert ballot_array_props.safe_is_safe)
+  apply (auto simp add:agreement_def)
+  using ballot_array_props.intro quorums_axioms by fastforce
 
 end
