Isabelle2/AbstractMultiPaxos5.thy
@@ -7,13 +7,14 @@ begin
 datatype ('v,'a,'l) amp_action =
   Propose 'v
 | Learn nat 'v 'l
-| Vote 
-| JoinBallot
+| Vote 'a "'a fset" nat 'v 
+  -- {* an acceptor votes in a ballot according to a quorum *}
+| JoinBallot 'a nat
 
 record ('v,'a) amp_state =
   propCmd :: "'v fset"
   ballot :: "'a \<Rightarrow> nat option"
-  vote :: "'a \<Rightarrow> nat \<Rightarrow> nat \<Rightarrow> 'v option"
+  vote :: "nat \<Rightarrow> 'a \<Rightarrow> nat \<Rightarrow> 'v option"
 
 text {* We give all the parameters in order to fix their type. Also fixed ballots to be nat. *}
 locale abs_multi_paxos = IOA + quorums +
@@ -23,34 +24,47 @@ begin
 
 definition amp_asig where
   "amp_asig \<equiv>
-    \<lparr> inputs = { a . \<exists> c . a = Propose c  },
-      outputs = { a . \<exists> v l i . l |\<in>| learners \<and> a = Learn i v l },
-      internals = {Vote} \<union> {JoinBallot}\<rparr>"
+    \<lparr> inputs = { Propose c | c . True},
+      outputs = { Learn i v l | i v l . l |\<in>| learners},
+      internals = {Vote a i q b | a i b q . a |\<in>| acceptors} \<union> {JoinBallot a b | a b . a |\<in>| acceptors}\<rparr>"
 
 definition amp_start where
-  "amp_start \<equiv> {\<lparr>propCmd = {||}, ballot = (\<lambda> a . None), vote = (\<lambda> a i b . None) \<rparr>}"
+  "amp_start \<equiv> {\<lparr>propCmd = {||}, ballot = (\<lambda> a . None), vote = (\<lambda> i a b . None) \<rparr>}"
 
 definition propose where
   "propose c r r' \<equiv> (r' = r\<lparr>propCmd := (propCmd r) |\<union>| {|c|}\<rparr>)"
 
 definition join_ballot where
-  "join_ballot s s' \<equiv> 
-    \<exists> a b . a |\<in>| acceptors \<and> Some b > (ballot s a) \<and> s' = s\<lparr>ballot := (ballot s)(a := Some b)\<rparr>"
+  "join_ballot a b s s' \<equiv> 
+    a |\<in>| acceptors \<and> Some b > (ballot s a) \<and> s' = s\<lparr>ballot := (ballot s)(a := Some b)\<rparr>"
+
+abbreviation proved_safe_at where 
+  -- {* v is proved safe in instance i at ballot b by quorum q *}
+  "proved_safe_at s i q b v \<equiv> ballot_array.proved_safe_at  (vote s i) q b v"
+abbreviation conservative_at where 
+  "conservative_at s i \<equiv> ballot_array.conservative_array (vote s i) acceptors"
 
 definition do_vote where
-  "do_vote s s' \<equiv> \<exists> a i . a |\<in>| acceptors \<and> (let bo = ballot s a; b = the bo in
-        bo \<noteq> None \<and> (\<exists> v . ballot_array.proved_safe_at  (\<lambda> a . vote s a i) acceptors b v 
-        \<and> ballot_array.conservative_array  (\<lambda> a . vote s' a i) acceptors
-        \<and> vote s a i b = None \<and> s' = s\<lparr>vote := (vote s)(a := (vote s a)(i := 
-            (vote s a i)(b := Some v)))\<rparr>))"
+  "do_vote a i q v s s' \<equiv> a |\<in>| acceptors \<and> (case ballot s a of None \<Rightarrow> False | Some b \<Rightarrow> 
+        proved_safe_at s i q b v 
+        \<and> q |\<in>| quorums
+        \<and> (\<forall> a2 . a2 |\<in>| q \<longrightarrow> ballot s a2 \<ge> Some b)
+        \<and> conservative_at s' i
+        \<and> vote s i a b = None 
+        \<and> s' = s\<lparr>vote := (vote s)(i := (vote s i)(a := 
+            (vote s i a)(b := Some v)))\<rparr>)"
 
+abbreviation chosen where 
+  "chosen s i v \<equiv> ballot_array.chosen (vote s i) quorums v"
 definition learn where
-  "learn l i v s s' \<equiv> ((ballot_array.chosen (\<lambda> a . vote s a i) quorums) v) \<and> s = s'"
+  "learn l i v s s' \<equiv> chosen s i v \<and> s = s'"
 
+(* Here it's better to have all existentially quantified parameters in the action itself, in
+  order to avoid annoying quantifiers. *)
 fun amp_trans_fun  where
   "amp_trans_fun r (Propose c) r' = propose c r r'"
-| "amp_trans_fun r JoinBallot r' = join_ballot r r'"
-| "amp_trans_fun r Vote r' = do_vote r r'"
+| "amp_trans_fun r (JoinBallot a b) r' = join_ballot a b r r'"
+| "amp_trans_fun r (Vote a q i v) r' = do_vote a i q v r r'"
 | "amp_trans_fun r (Learn i v l) r' = learn l i v r r'"
 
 definition amp_trans where
@@ -77,9 +91,23 @@ declare the_ioa_def[inv_proofs_defs]
 declare propose_def[simp] join_ballot_def[simp] do_vote_def[simp]
   learn_def[simp]
 
+lemma vote_one_inst_only:
+  assumes "do_vote a i q v s s'" and "i \<noteq> j"
+  shows "vote s j a = vote s' j a "
+using assms
+apply auto
+    apply (case_tac "ballot s a")
+apply auto
+done
+
+lemma vote_ballot_unch:
+  assumes "do_vote a i q v s s'"
+  shows "ballot s = ballot s'"
+using assms by (auto split add:option.split_asm)
+
 declare ballot_array.conservative_array_def[inv_proofs_defs]
 abbreviation conservative_array where 
-"conservative_array s \<equiv>  \<forall> i . ballot_array.conservative_array (\<lambda> a . vote s a i) acceptors"
+"conservative_array s \<equiv>  \<forall> i . conservative_at s i"
 lemma conservative_inductive:
   "invariant the_ioa conservative_array"
 apply (try_solve_inv2 inv_proofs_defs:inv_proofs_defs invs:invs)
@@ -90,146 +118,127 @@ apply (try_solve_inv2 inv_proofs_defs:inv_proofs_defs invs:invs)
     defer
     apply (force simp add:inv_proofs_defs)
   apply (match premises in R[thin]:"reachable ?ioa ?s" \<Rightarrow> \<open>-\<close>)
-  subgoal premises prems for s t a using prems
+  subgoal premises prems for s t act a q i v using prems
   proof -
-    from prems(2,3) 
-    obtain a i where 1:"a |\<in>| acceptors \<and> (let bo = ballot s a; b = the bo in
-        bo \<noteq> None \<and> (\<exists> v . ballot_array.proved_safe_at  (\<lambda> a . vote s a i) acceptors b v 
-        \<and> ballot_array.conservative_array  (\<lambda> a . vote t a i) acceptors
-        \<and> vote s a i b = None \<and> t = s\<lparr>vote := (vote s)(a := (vote s a)(i := 
-            (vote s a i)(b := Some v)))\<rparr>))"
-    by (auto simp add:inv_proofs_defs)
+    from prems(2,3)
+    obtain b where 1:"a |\<in>| acceptors" and 2:"ballot s a = Some b" 
+    and 3:"proved_safe_at s i q b v"
+    and 6:"ballot_array.conservative_array  (vote t i) acceptors"
+    and 4:"vote s i a b = None" and 5:"t = s\<lparr>vote := (vote s)(i := (vote s i)(a := (vote s i a)(b := Some v)))\<rparr>"
+        apply (case_tac "ballot s a")
+          by (auto simp add:inv_proofs_defs)
     show "conservative_array t"
     proof (auto simp add: ballot_array.conservative_array_def)
       fix j b
-      have "ballot_array.conservative (\<lambda>a. vote t a j) acceptors b" if "i \<noteq> j" 
+      have "ballot_array.conservative (vote t j) acceptors b" if "i \<noteq> j"
       proof -
-        have "ballot_array.conservative (\<lambda>a. vote s a j) acceptors b" using prems(1)
+        have "ballot_array.conservative (vote s j) acceptors b" using prems(1)
           by (auto simp add: ballot_array.conservative_array_def ballot_array.conservative_def)
-        moreover from 1 obtain v where "t = s\<lparr>vote := (vote s)(a := (vote s a)(i :=
-            (vote s a i)((the (ballot s a)) := Some v)))\<rparr>" by meson
-        ultimately show ?thesis using that by (auto simp add:ballot_array.conservative_def)
+        thus ?thesis using that 5 by (auto simp add: ballot_array.conservative_def)
       qed
       moreover
-      have "ballot_array.conservative (\<lambda>a. vote t a j) acceptors b" if "i = j"
-        using 1 that by auto (metis ballot_array.conservative_array_def) 
-      ultimately show "ballot_array.conservative (\<lambda>a. vote t a j) acceptors b" by auto
+      have "ballot_array.conservative (vote t j) acceptors b" if "i = j"
+        using 6 that by auto (metis ballot_array.conservative_array_def)
+      ultimately show "ballot_array.conservative (vote t j) acceptors b" by auto
     qed
   qed 
 done
 declare conservative_inductive[invs]
 
-(*
-abbreviation safe_at where "safe_at \<equiv> \<lambda> s . ballot_array.safe_at (ballot s) (vote s) quorums"
+abbreviation safe_at where "safe_at s i \<equiv> ballot_array.safe_at (ballot s) (vote s i) quorums"
 lemma safe_mono:
-  assumes "safe_at s v b" and "s \<midarrow>a\<midarrow>the_ioa\<longrightarrow> t"
-  shows "safe_at t v b" using assms oops
+  assumes "safe_at s i v b" and "s \<midarrow>a\<midarrow>the_ioa\<longrightarrow> t"
+  shows "safe_at t i v b" using assms
 apply (cases a)
-        apply (auto simp add:inv_proofs_defs ballot_array.safe_at_def ballot_array.choosable_def)[2] (* propose, learn *)
-    defer (* join_ballot *)
+         (* propose, learn *)
+        apply (auto simp add:inv_proofs_defs ballot_array.safe_at_def ballot_array.choosable_def)[2]
+    defer 
+    (* join_ballot *)
     apply (simp add:inv_proofs_defs ballot_array.safe_at_def ballot_array.choosable_def)[1]
-    apply (metis less_def order.strict_trans) 
-  defer (* vote *)
-  apply (simp add:inv_proofs_defs ballot_array.safe_at_def ballot_array.choosable_def)
-  apply (smt fun_upd_apply neq_iff option.sel p_state.select_convs(2) p_state.select_convs(3) p_state.surjective p_state.update_convs(3))
-  (* That was amazing, Sledgehammer found it before I had time to think about why it would be true... *)
-apply (simp add:inv_proofs_defs ballot_array.safe_at_def ballot_array.choosable_def) (* start_ballot *)
-apply (metis p_state.ext_inject p_state.surjective p_state.update_convs(4))
+    apply (metis less_def order.strict_trans)
+  (* vote *)
+  apply (simp add:inv_proofs_defs ballot_array.safe_at_def ballot_array.choosable_def split add:option.split_asm)
+  apply (metis neq_iff)
 done
 
-abbreviation safe where "safe \<equiv> \<lambda> s . ballot_array.safe (ballot s) (vote s) quorums acceptors"
-definition inv2 where
-  "inv2 s \<equiv> safe s \<and> (\<forall> b . case suggestion s b of None \<Rightarrow> True | Some v \<Rightarrow> safe_at s v b)"
-declare inv2_def[inv_proofs_defs]
-
-lemma inv2:
-  "invariant the_ioa inv2"
+abbreviation safe where "safe s \<equiv> \<forall> i . ballot_array.safe (ballot s) (vote s i) quorums acceptors"
+lemma safe_inv:
+  "invariant the_ioa safe"
 apply(rule invariantI)
-    apply (force simp add:inv_proofs_defs ballot_array.safe_def)
+    apply (force simp add:ballot_array.safe_def inv_proofs_defs)
   apply instantiate_invs_2
   apply (case_tac a)
-          subgoal premises prems for s t a v
-          proof -
-            from prems(2,7) have 1:"propose v s t"
-              by (auto simp add:inv_proofs_defs) 
-            hence 2:"\<And> b . suggestion s b = suggestion t b" 
-              by(auto simp add:inv_proofs_defs)
-            have 3:"safe t" using 1 prems(1) 
-              by (auto simp add:inv_proofs_defs ballot_array.safe_def ballot_array.safe_at_def ballot_array.choosable_def) 
-            from 1 2 3 safe_mono show ?thesis 
-              by (auto simp add:inv2_def)
-                (metis inv2_def option.case_eq_if prems(1) prems(2))
-          qed
-        subgoal by (auto simp add:inv_proofs_defs) (* learn *)
-      subgoal premises prems for s t act a
-      proof - 
-        from prems(2,7) have 1:"do_vote a s t"
-          by(auto simp add:inv_proofs_defs)
-        hence 2:"\<And> b . suggestion s b = suggestion t b" 
-          by (auto simp add:inv_proofs_defs)
-            (metis p_state.ext_inject p_state.surjective p_state.update_convs(3))
-        have 3:"safe t" using prems(1) 1 apply(auto simp add:inv2_def ballot_array.safe_def)
-          proof - (* Auto-generated by Sledgehammer *)
-            fix b :: nat and aa :: 'a
-            assume a1: "aa |\<in>| acceptors"
-            assume a2: "let bo = ballot s a; b = the bo in (\<exists>y. bo = Some y) \<and> vote s a b = None \<and> t = s \<lparr>vote := (vote s)(a := (vote s a)(b := suggestion s b))\<rparr>"
-            assume a3: "\<forall>b. case suggestion s b of None \<Rightarrow> True | Some v \<Rightarrow> safe_at s v b"
-            assume a4: "\<forall>b a. a |\<in>| acceptors \<longrightarrow> (let vote = vote s a b in (\<exists>y. vote = Some y) \<longrightarrow> safe_at s (the vote) b)"
-            { fix vv :: 'v
-              have ff1: "\<And>n. suggestion s n = None \<or> safe_at s (the (suggestion s n)) n"
-                using a3 by (metis option.case_eq_if)
-              obtain nn :: nat where
-                ff2: "s\<lparr>vote := (vote s) (a := (vote s a) (the (ballot s a) := suggestion s (the (ballot s a))))\<rparr> = t \<and> ballot s a = Some nn \<and> vote s a (the (ballot s a)) = None"
-                using a2 by metis
-              have "\<forall>p. \<exists>f fa fb fc u. \<lparr>propCmd = f::'v fset, ballot = fa::'a \<Rightarrow> nat option, vote = fb, suggestion = fc, \<dots> = u::unit\<rparr> = p"
-                by (metis p_state.cases_scheme)
-              then obtain ff :: "('v, 'a) p_state \<Rightarrow> 'v fset" and zz :: "('v, 'a) p_state \<Rightarrow> 'a \<Rightarrow> nat option" and zza :: "('v, 'a) p_state \<Rightarrow> 'a \<Rightarrow> nat \<Rightarrow> 'v option" and zzb :: "('v, 'a) p_state \<Rightarrow> nat \<Rightarrow> 'v option" and uu :: "('v, 'a) p_state \<Rightarrow> unit" where
-                ff3: "\<And>p. \<lparr>propCmd = ff p, ballot = zz p, vote = zza p, suggestion = zzb p, \<dots> = uu p\<rparr> = p"
-                by moura
-              then have ff4: "\<And>p. vote p = zza p"
-                by (metis p_state.select_convs(3))
-              have "(zza s)(a := (zza s a)(the (Some nn) := suggestion s (the (Some nn)))) = zza t"
-                using ff3 ff2 by (metis p_state.select_convs(3) p_state.update_convs(3))
-              then have "zza t aa b = Some vv \<longrightarrow> ballot_array.safe_at (ballot s) (zza s) quorums (the (Some vv)) b"
-                using ff4 ff2 ff1 a4 a1 by (metis fun_upd_apply)
-              then have "vote t aa b \<noteq> Some vv \<or> safe_at t (the (vote t aa b)) b"
-                using ff4 by (metis prems(2) safe_mono) }
-            then show "let z = vote t aa b in (\<exists>v. z = Some v) \<longrightarrow> safe_at t (the z) b"
-              by metis
-          qed
-        from 1 2 3 safe_mono show ?thesis 
-          by (auto simp add:inv2_def)
-            (metis inv2_def option.case_eq_if prems(1) prems(2))
+        (* propose *)
+        apply (force simp add:ballot_array.safe_def inv_proofs_defs ballot_array.safe_at_def ballot_array.choosable_def)
+      (* learn *)
+      apply (force simp add:ballot_array.safe_def inv_proofs_defs ballot_array.safe_at_def ballot_array.choosable_def)
+    (* vote *)
+    subgoal premises prems for s t act a q i v
+    proof (auto simp add:ballot_array.safe_def Let_def split add:option.split)
+      fix j b a\<^sub>2 v\<^sub>2
+      assume 1:"a\<^sub>2 |\<in>| acceptors" and 2:"vote t j a\<^sub>2 b = Some v\<^sub>2"
+      have l:"safe_at t j v\<^sub>2 b" if  "vote s j a\<^sub>2 b = vote t j a\<^sub>2 b"
+      proof -
+        have "safe_at s j v\<^sub>2 b" using that 1 2 prems(1) by (simp add:ballot_array.safe_def split add:option.split_asm)
+        thus ?thesis using prems(2) safe_mono by blast
       qed
-    subgoal premises prems for s t act b a
-    proof -
-      from prems(2,7) have 1:"join_ballot a b s t"
-        by (auto simp add:inv_proofs_defs)
-      hence 2:"\<And> b . suggestion s b = suggestion t b" 
-        by (auto simp add:inv_proofs_defs)
-      have 3:"safe t" using prems(1) 1 apply (auto simp add:inv2_def ballot_array.safe_def)
-        by (metis p_state.ext_inject p_state.surjective p_state.update_convs(2) prems(2) safe_mono) 
-      from 1 2 3 safe_mono show ?thesis 
-        by (auto simp add:inv2_def)
-          (metis inv2_def option.case_eq_if prems(1) prems(2))
+      show "safe_at t j v\<^sub>2 b"
+      proof (cases "i = j \<and> a\<^sub>2 = a")
+      case False
+        have "vote s j a\<^sub>2 b = vote t j a\<^sub>2 b" using False prems(2,5) vote_one_inst_only
+          by (auto simp add:is_trans_def the_ioa_def amp_ioa_def amp_trans_def split add:option.split_asm)
+        with l show ?thesis by auto
+      next
+      case True
+        have 6:"do_vote a\<^sub>2 j q v s t" using prems(2,5) 1 True by (auto simp add:inv_proofs_defs)
+        with this obtain b\<^sub>2 where 3:"ballot s a\<^sub>2 = Some b\<^sub>2" and 4:"proved_safe_at s j q b\<^sub>2 v"
+        and 5:"t = s\<lparr>vote := (vote s)(j := (vote s j)(a\<^sub>2 := (vote s j a\<^sub>2)(b\<^sub>2 := Some v)))\<rparr>"
+        and 7:"\<And> a2 . a2 |\<in>| q \<Longrightarrow> ballot s a2 \<ge> Some b\<^sub>2" and 8:"q |\<in>| quorums"
+          by (auto split add:option.split_asm)
+        have ?thesis if "b \<noteq> b\<^sub>2"
+        proof -
+          have "vote s j a\<^sub>2 b = vote t j a\<^sub>2 b" using 5
+            by (smt amp_state.ext_inject amp_state.surjective amp_state.update_convs(3) fun_upd_apply that) 
+          with l show ?thesis by auto
+        qed
+        moreover have ?thesis if "b = b\<^sub>2"
+        proof -
+          have "v = v\<^sub>2" using that True
+            by (smt "2" "5" amp_state.ext_inject amp_state.surjective amp_state.update_convs(3) fun_upd_apply map_upd_Some_unfold)
+          hence 9:"vote t j a\<^sub>2 b = Some v\<^sub>2" using 5 that by force
+          hence "safe_at s j v\<^sub>2 b\<^sub>2" 
+            using ballot_array_props.proved_safe_is_safe[of quorums acceptors "ballot s" "(vote s j)" q b\<^sub>2 v] 4 3 7 8 prems(1,3) that `v = v\<^sub>2`
+            by auto (metis ballot_array_props_def quorums_axioms)
+          with safe_mono prems(2) that True show ?thesis by blast
+        qed
+        ultimately show ?thesis by auto
+      qed
     qed
-  subgoal premises prems for s t act b
-  proof -
-    from prems(2,7) have 1:"start_ballot b s t"
-      by(auto simp add:inv_proofs_defs)
-    have 3:"safe t" using prems(1) 1 by (auto simp add:inv2_def ballot_array.safe_def)
-    from 1 obtain q v where 2:"q |\<in>| quorums" and 4:"(ballot_array.proved_safe_at (vote s)) q b v" 
-      and 5:"t = s\<lparr>suggestion := suggestion s(b \<mapsto> v)\<rparr>" and 6:"\<And> a . a |\<in>| q \<Longrightarrow> ballot s a \<ge> Some b"
-      by auto
-    interpret ba_props:ballot_array_props "ballot s" "vote s" by unfold_locales
-    have 2:"\<And> b . case suggestion t b of None \<Rightarrow> True | Some v \<Rightarrow> safe_at t v b"
-      using 1 2 4 5 6 prems(1,2,3)
-        by (simp add:inv2_def)
-          (simp add: ba_props.proved_safe_is_safe option.case_eq_if prems(4))
-    from 2 3 show ?thesis by (auto simp add:inv2_def)
+  (* join_ballot *)
+  subgoal premises prems for s t act a b
+  proof (auto simp add:ballot_array.safe_def split add:option.split)
+    fix i b\<^sub>2 a\<^sub>2 v
+    assume "vote t i a\<^sub>2 b\<^sub>2 = Some v" and "a\<^sub>2 |\<in>| acceptors"
+    note 1 = this
+    have 2:"vote t i a\<^sub>2 b\<^sub>2 = vote s i a\<^sub>2 b\<^sub>2" using prems(2,5) by (auto simp add:inv_proofs_defs)
+    hence 3:"safe_at s i v b\<^sub>2" using 1 prems(1)
+      by (metis ballot_array.safe_def option.simps(5)) 
+    with safe_mono prems(2,5)
+    show "safe_at t i v b\<^sub>2" apply (auto simp add:inv_proofs_defs)
+      by (metis amp_proof.safe_mono amp_proof_axioms amp_state.select_convs(3) amp_state.simps(2) amp_state.surjective amp_state.update_convs(2) prems(2) the_ioa_def) 
   qed
 done
-declare inv2[invs]
-*)
+declare safe_inv[invs]
+
+definition agreement where 
+  "agreement s \<equiv> \<forall> v w i . chosen s i v \<and> chosen s i w \<longrightarrow> v = w"
+lemma agreement:"invariant the_ioa agreement"
+apply(rule invariantI)
+    apply(auto simp add: inv_proofs_defs agreement_def ballot_array.chosen_def ballot_array.chosen_at_def)[1]
+    apply (metis fempty_iff quorum_inter_witness)
+  apply instantiate_invs_2
+  apply (insert ballot_array_props.safe_is_safe)
+  apply (auto simp add:agreement_def)
+  using ballot_array_props.intro quorums_axioms by fastforce
 
 end
